CC/Reduction/Preservation.lean
@@ -14,21 +14,22 @@ import CC.Reduction
 import CC.StoreContext.Lookup
 import CC.Typed.Basic
 import CC.Typed.Opening
+import CC.Subtype.Subst
 
 namespace CC
 
-inductive Match : CType n1 m1 -> CType n2 m2 -> Prop where
+inductive Match : Ctx n1 m1 -> CType n1 m1 -> Ctx n2 m2 -> CType n2 m2 -> Prop where
 | same :
-  Match T T
+  Match Γ T Γ T
 | weaken :
-  Match T.weaken_var T
+  Match Γ T (Ctx.extend_var Γ P) T.weaken_var
 
 theorem preservation :
-  TypedState st1 T1 ->
+  TypedState st1 Γ1 T1 ->
   Reduce st1 st2 ->
-  ∃ T2, TypedState st2 T2 ∧ Match T1 T2 := by
+  ∃ Γ2 T2, TypedState st2 Γ2 T2 ∧ Match Γ1 T1 Γ2 T2 := by
   intro ht hr
-  induction hr
+  induction hr generalizing T1
   case red_app hl =>
     cases ht; rename_i hs hv
     have h1 := Typed.app_inv hv
@@ -38,7 +39,7 @@ theorem preservation :
     have h3 := Typed.var_typing_captures hy
     subst_vars
     have h4 := Typed.open_var hy ht
-    apply Exists.intro T1
+    apply Exists.intro Γ1; apply Exists.intro T1
     constructor
     constructor; trivial
     apply Typed.sub
@@ -52,7 +53,7 @@ theorem preservation :
     have h2 := lookup_tfun hs hx hl
     let ⟨C2, ht⟩ := h2
     have h3 := Typed.open_tvar SubtypeP.refl ht
-    apply Exists.intro T1
+    apply Exists.intro Γ1; apply Exists.intro T1
     constructor
     constructor; trivial
     apply Typed.sub
@@ -66,11 +67,71 @@ theorem preservation :
       let ⟨Cx, Cf, hx⟩ := h1
       have h2 := lookup_box hs hx hl
       let ⟨C2, hy⟩ := h2
-      apply Exists.intro T1
+      apply Exists.intro Γ1; apply Exists.intro T1
       constructor
       constructor; trivial
       trivial
       constructor
-  case red_rename => sorry
-  case red_liftval => sorry
-  case red_ctx => sorry
+  case red_rename =>
+    let ⟨hs, hv⟩ := ht
+    have h1 := Typed.let_inv hv
+    let ⟨Ct, Cu, T, U0, U1, hx, ht, heq, hs, _⟩ := h1
+    cases heq
+    have h2 := Typed.var_typing_captures hx
+    cases h2
+    have h3 := Typed.open_var hx ht
+    unfold CType.open_var at h3
+    unfold CType.weaken_var at h3
+    simp [CType.rename_comp] at h3
+    apply Exists.intro Γ1; apply Exists.intro T1
+    apply And.intro
+    constructor; trivial
+    apply Typed.sub <;> assumption
+    constructor
+  case red_liftval t v =>
+    let ⟨hs, hv⟩ := ht
+    have h1 := Typed.let_inv hv
+    let ⟨Ct, Cu, T, U0, U1, hx, ht, heq, hs, hh⟩ := h1
+    cases heq
+    apply Exists.intro; apply Exists.intro T1.weaken_var
+    constructor
+    constructor
+    constructor <;> trivial
+    apply Typed.sub
+    trivial
+    apply Subtype.weaken_var; trivial
+    constructor
+  case red_ctx1 ih =>
+    let ⟨hts, hv⟩ := ht 
+    have h1 := Typed.let_inv hv
+    let ⟨Ct, Cu, T, U0, U1, ht, hu, heq, hsub, hh, hh1⟩ := h1
+    cases heq
+    have hts' := TypedState.state hts ht
+    have ih' := ih hts'
+    let ⟨Γ2, T2, ⟨hts'', ht'⟩, hm⟩ := ih'
+    cases hm with
+    | same => 
+      have ⟨C', hh'⟩ := hh _ _ ht'
+      have h0 := TypedState.state hts'' hh'
+      apply Exists.intro Γ1
+      apply Exists.intro T1
+      apply And.intro
+      · assumption
+      · constructor 
+  case red_ctx2 ih =>
+    let ⟨hts, hv⟩ := ht
+    have h1 := Typed.let_inv hv
+    let ⟨Ct, Cu, T, U0, U1, ht, hu, heq, hsub, hh, hh1⟩ := h1
+    cases heq
+    have hts' := TypedState.state hts ht
+    have ih' := ih hts'
+    let ⟨Γ2, T2, ⟨hts'', ht'⟩, hm⟩ := ih'
+    cases hm with
+    | weaken => 
+      rename_i P0
+      have ⟨C', hh'⟩ := hh1 _ _ P0 ht'
+      have h0 := TypedState.state hts'' hh'
+      repeat apply Exists.intro
+      apply And.intro
+      · exact h0
+      · constructor
